WIP symex
wf_iter_step_constructive

minuska/theories/symex.v
@@ -2,3 +2,211 @@ From Minuska Require Import
     prelude
     spec
 .
+
+From CoLoR Require
+    Term.WithArity.ASignature
+    Term.WithArity.AUnif
+.
+
+Definition Satisfies_variable_GroundTerm'
+    {Σ : StaticModel}
+    (ρ : Valuation2)
+    (t : TermOver builtin_value)
+    (x : variable)
+    := ρ !! x = Some t
+.
+
+#[export]
+Instance Satisfies_variable_GroundTerm
+    {Σ : StaticModel}
+    : Satisfies
+        Valuation2
+        (TermOver builtin_value)
+        variable
+        variable
+:= {|
+    satisfies :=
+        fun
+            (ρ : Valuation2)
+            (t : TermOver builtin_value)
+            (x : variable) => Satisfies_variable_GroundTerm' ρ t x
+|}.
+
+
+Equations? sat2v
+    {Σ : StaticModel}
+    (ρ : Valuation2)
+    (t : TermOver builtin_value)
+    (φ : TermOver variable)
+    : Prop
+    by wf (TermOver_size φ) lt
+:=
+    sat2v ρ t (t_over x) := Satisfies_variable_GroundTerm' ρ t x ;
+    sat2v ρ (t_over _) (t_term s l) := False ;
+    sat2v ρ (t_term s' l') (t_term s l) :=
+        ((s' = s) /\
+        (length l' = length l) /\
+        forall i t' φ' (pf1 : l !! i = Some φ') (pf2 : l' !! i = Some t'),
+            sat2v ρ t' φ'
+        )
+    ;
+.
+Proof.
+    abstract(
+    unfold satisfies in *; simpl in *;
+    simpl;
+    apply take_drop_middle in pf1;
+    rewrite <- pf1;
+    rewrite sum_list_with_app; simpl;
+    ltac1:(lia)).
+Defined.
+
+#[export]
+Instance Satisfies_TOV_GroundTerm
+    {Σ : StaticModel}
+    : Satisfies
+        Valuation2
+        (TermOver builtin_value)
+        (TermOver variable)
+        variable
+:= {|
+    satisfies := fun ρ g φ => sat2v ρ g φ
+|}.
+
+Record SymCfg {Σ : StaticModel} := {
+    scfg_pattern : TermOver variable ;
+    scfg_side_conditions : list SideCondition2 ;
+}.
+
+Definition Satisfies_SymCfg_GroundTerm'
+    {Σ : StaticModel}
+    (ρ : Valuation2)
+    (g : TermOver builtin_value)
+    (scfg : SymCfg)
+:=
+    ((satisfies ρ g scfg.(scfg_pattern))
+    * (satisfies ρ tt scfg.(scfg_side_conditions)))%type
+.
+
+#[export]
+Instance Satisfies_SymCfg_GroundTerm
+    {Σ : StaticModel}
+    : Satisfies
+        Valuation2
+        (TermOver builtin_value)
+        (SymCfg)
+        variable
+:= {|
+    satisfies := fun ρ g φ => Satisfies_SymCfg_GroundTerm' ρ g φ
+|}.
+
+Definition Satisfies_listSymCfg_GroundTerm'
+    {Σ : StaticModel}
+    (ρ : Valuation2)
+    (g : TermOver builtin_value)
+    (lφ : list SymCfg)
+:=
+    forall φ, φ ∈ lφ -> satisfies ρ g φ
+.
+
+#[export]
+Instance Satisfies_listSymCfg_GroundTerm
+    {Σ : StaticModel}
+    : Satisfies
+        Valuation2
+        (TermOver builtin_value)
+        (list SymCfg)
+        variable
+:= {|
+    satisfies := Satisfies_listSymCfg_GroundTerm'
+|}.
+
+Definition SymexStep {Σ : StaticModel}
+:=
+    SymCfg -> list SymCfg
+.
+
+Definition SymexStep_correct
+    {Σ : StaticModel}
+    (Act : Set)
+    (Γ : RewritingTheory2 Act)
+    (step : SymexStep)
+:=
+    ∀ (φ : SymCfg) (g : TermOver builtin_value),
+        ( { ρ : Valuation2 & satisfies ρ g φ} ) ->
+        ∀ (g' : TermOver builtin_value),
+        ((
+            ({ ρ : Valuation2 & satisfies ρ g' (step φ)} )
+            ->
+            (rewriting_relation Γ g g')
+        )
+        *
+        (
+            (rewriting_relation Γ g g') ->
+            ({ ρ : Valuation2 & satisfies ρ g' (step φ)} )
+        ))%type
+
+.
+
+Program Definition ColorSignatureOf (Σ : StaticModel)
+    : Term.WithArity.ASignature.Signature
+:= {|
+    Term.WithArity.ASignature.symbol := (nat*(@spec.symbol Σ)) ;
+    Term.WithArity.ASignature.arity := fun ns => ns.1 ;
+    Term.WithArity.ASignature.beq_symb :=
+        fun s1 s2 => bool_decide (s1 = s2) ;
+|}.
+Next Obligation.
+    abstract(
+        assert (H := bool_decide_spec ((n0,s0)=(n,s)));
+        unfold Is_true in H;
+        ltac1:(case_match; naive_solver)
+    ).
+Defined.
+Fail Next Obligation.
+
+
+Lemma wf_iter_step_constructive
+    {Σ' : Term.WithArity.ASignature.Signature}
+    (p : @Term.WithArity.AUnif.problem Σ')
+ :
+    { k : nat & @Term.WithArity.AUnif.solved Σ' (Term.WithArity.AUnif.iter_step k p) = true }.
+Proof. 
+    assert (HH := (Term.WithArity.AUnif.wf_Lt' p)).
+    induction HH.
+    {
+        destruct x.
+        {
+            destruct p.
+            destruct e; simpl in *.
+            { exists 0. reflexivity. }
+            {
+                remember (Some (s, e::e0)) as p.
+                destruct (Term.WithArity.AUnif.solved (Term.WithArity.AUnif.step p)) eqn:Heqsolved.
+                {
+                    exists 1. simpl.
+                    ltac1:(repeat (case_match; simpl in *; simplify_eq/=; try reflexivity)).
+                }
+                {
+                    specialize (X (Term.WithArity.AUnif.step p)).
+                    
+                    ltac1:(ospecialize (X _)).
+                    {
+                        assert(Htmp := (Term.WithArity.AUnif.Lt_step _ (Term.WithArity.AUnif.solved_inv _ Heqsolved))).
+                        subst p. exact Htmp.
+                    }
+                    destruct X as [k Hk].
+                    exists (S k). simpl.
+                    rewrite <- Term.WithArity.AUnif.iter_step_commut.
+                    subst p.
+                    exact Hk.
+                }
+            }
+        }
+        {
+            exists 0. reflexivity.
+        }
+    }
+ Qed.
+
+
