minuska/theories/spec_interpreter.v
@@ -4,16 +4,6 @@ From Minuska Require Import
 .
 
 
-
-Definition rewriting_relation
-    {Σ : StaticModel}
-    {Act : Set}
-    (Γ : list (RewritingRule2 Act))
-    : TermOver builtin_value -> TermOver builtin_value -> Type
-    := fun from to =>
-        { r : _ & { a : _ & ((r ∈ Γ) * rewrites_to r from a to)%type}}
-.
-
 Definition not_stuck
     {Σ : StaticModel}
     {Act : Set}
